iAAHHH

ulib/experimental/Steel.Effect.Atomic.fst
@@ -49,6 +49,136 @@ let new_invariant i p = SteelAtomic?.reflect (Steel.Memory.new_invariant i p)
 let with_invariant i f = SteelAtomic?.reflect (Steel.Memory.with_invariant i (reify (f())))
 let frame frame f = SteelAtomic?.reflect (Steel.Memory.frame frame (reify (f ())))
 let change_slprop p q proof = SteelAtomic?.reflect (Steel.Memory.change_slprop p q proof)
-let witness_h_exists = admit()
+
+open NMSTTotal
+open MSTTotal
+
+let not_affine (p : slprop) = forall m1 m2. interp p m1 ==> interp p m2 ==> m1 == m2
+
+val intro_star_pat (p q:slprop) (mp:hmem p) (mq:hmem q)
+  : Lemma
+    (requires disjoint mp mq)
+    (ensures interp (p `star` q) (join mp mq))
+    [SMTPat (interp (p `star` q) (join mp mq))]
+let intro_star_pat = intro_star
+
+val elim_star_pat (p q:slprop) (m:hmem (p `star` q))
+  : Lemma
+    (requires
+      interp (p `star` q) m)
+    (ensures exists ml mr.
+      disjoint ml mr /\ m == join ml mr /\ interp p ml /\ interp q mr)
+    [SMTPat (interp (p `star` q) m)]
+let elim_star_pat = elim_star
+
+let witness_h_exists (#a:Type) (#opened:_) (#p:a -> slprop) (_:unit)
+  : SteelAtomic (Ghost.erased a) opened unobservable
+                (h_exists p) (fun x -> p x)
+  =
+  SteelAtomic?.reflect begin
+  let pre m0 =
+    inames_ok opened m0
+    /\ interp (h_exists p `star` locks_invariant opened m0) m0
+  in
+  let post m0 (x:Ghost.erased a) m1 =
+    inames_ok opened m1
+    /\ interp (p x `star` locks_invariant opened m1) m1
+    /\ preserves_frame opened (h_exists p) (p x) m0 m1
+  in
+  let postn m0 (xn:(Ghost.erased a & nat)) m1 =
+    post m0 (fst xn) m1
+  in
+  let body7 (tpn:tape&nat) (m0:mem) : PURE ((Ghost.erased a & nat) & mem)
+                                         (fun p -> pre m0 /\
+                                                (forall (x:(Ghost.erased a & nat)) (m1:mem).
+                                                  postn m0 x m1 /\ mem_evolves m0 m1 ==> p (x,m1)))
+  =
+
+
+
+//let star (p1 p2: slprop u#a) : slprop u#a =
+//  fun (h: heap) -> exists (h1 h2 : heap).
+//        h1 `disjoint` h2 /\
+//        h == join h1 h2 /\
+//        interp p1 h1 /\
+//        interp p2 h2
+
+    let tp, n = tpn in
+    assert (interp (h_exists p `star` locks_invariant opened m0) m0);
+    let starprop (ml mr : mem) = ml `disjoint` mr /\
+                         m0 == join ml mr /\
+                         interp (h_exists p) ml /\
+                         interp (locks_invariant opened m0) mr
+    in
+    elim_star (h_exists p) (locks_invariant opened m0) m0;
+    let starprop1 ml : prop = exists mr. starprop ml mr in // this prop annotation seems needed
+    let ml : Ghost.erased mem = FStar.IndefiniteDescription.indefinite_description_tot mem starprop1 in
+    assert (starprop1 ml);
+    let starpropml mr : prop = starprop ml mr in
+    assert (exists mr. starpropml mr);
+    let mr : Ghost.erased mem = FStar.IndefiniteDescription.indefinite_description_tot mem starpropml in
+    assert (interp (h_exists p) ml /\ interp (locks_invariant opened m0) mr);
+    assert (interp (h_exists p) ml);
+    Steel.Memory.elim_h_exists p ml;
+    assert (exists x. interp (p x) ml);
+    let x = FStar.IndefiniteDescription.indefinite_description_tot a (fun x -> interp (p x) ml) in
+    assert (interp (p x) ml);
+    assert (interp (p x) ml /\ interp (locks_invariant opened m0) mr);
+    Steel.Memory.intro_star (p x) (locks_invariant opened m0) ml mr;
+    // COULD THIS HELP?
+    assume (forall x y m. interp (p x) m /\ interp (p y) m ==> x == y);
+    let key0 (m :mem) : Lemma (requires interp (h_exists p) m)
+                              (ensures (interp (p x) m)) =
+        Steel.Memory.elim_h_exists p m;
+        assert (exists y. interp (p y) m);
+        let y = FStar.IndefiniteDescription.indefinite_description_tot a
+                 (fun y -> interp (p y) m) in
+        assert (interp (p y) m);
+        assume (interp (p x) m);
+        ()
+    in
+    let key () : Lemma (forall m. interp (h_exists p) m ==> interp (p x) m) =
+      Classical.forall_intro (Classical.move_requires key0)
+    in
+    admit ();
+    key ();
+    let sub (frame:slprop)
+      : Lemma (requires (interp ((h_exists p `star` frame) `star` locks_invariant opened m0) m0))
+              (ensures  (interp ((p x        `star` frame) `star` locks_invariant opened m0) m0))
+      =
+           elim_star (h_exists p `star` frame) (locks_invariant opened m0) m0;
+           admit ()
+    in
+    Classical.forall_intro (Classical.move_requires sub);
+    assert (forall frame.
+             (interp ((h_exists p `star` frame) `star` locks_invariant opened m0) m0)
+             ==>
+             (interp ((p x `star` frame) `star` locks_invariant opened m0)) m0);
+    assert (preserves_frame opened (h_exists p) (p x) m0 m0);
+    assert (interp (p x `star` locks_invariant opened m0) m0);
+    ((x, n), m0)
+  in
+  let body8 (tpn:tape&nat) : MSTATETOT (Ghost.erased a & nat) mem mem_evolves
+                                (requires pre)
+                                (ensures postn)
+  =
+     MSTATETOT?.reflect (body7 tpn)
+  in
+  let body9 : NMSTTotal.repr (Ghost.erased a)
+                                mem mem_evolves
+                                (requires pre)
+                                (ensures post)
+  =
+      body8
+  in
+  let body10 () : MstTot (Ghost.erased a) opened (h_exists p) (fun x -> p x) =
+    NMSTATETOT?.reflect body9
+  in
+  let act : atomic_repr (Ghost.erased a) opened unobservable (h_exists p) (fun x -> p x) =
+    body10
+  in
+  act
+  end
+
 let lift_h_exists_atomic #a #u p = SteelAtomic?.reflect (Steel.Memory.lift_h_exists #u p)
 let elim_pure #uses p = SteelAtomic?.reflect (Steel.Memory.elim_pure #uses p)
